work on IF part

model/agp32RelationScript.sml
@@ -85,8 +85,9 @@ End
 (* relation between the pipelined Silver circuit and ISA state *)
 Definition IF_Rel_def:
   IF_Rel (fext:ext) (s:state_circuit) (a:ag32_state) (i:num) <=>
-  ((fext.ready ==> s.IF.IF_instr = instr (FUNPOW Next (i-1) a)) /\
-   (~fext.ready ==> s.IF.IF_instr = 63w))
+  (fext.ready ==> s.IF.IF_instr = instr (FUNPOW Next (i-1) a)) /\
+  (~fext.ready ==> s.IF.IF_instr = 63w) /\
+  (s.PC = (FUNPOW Next (i-1) a).PC)
 End
 
 Definition ID_Rel_def:
@@ -217,8 +218,9 @@ Definition WB_Rel_def:
 End
 
 (* TODO: refine the definition *)
+(* si: circuit state at cycle t-1 *)
 Definition Rel_def:
-  Rel (I:num # num -> num) (fext:ext) (s:state_circuit) (a:ag32_state) (t:num) <=>
+  Rel (I:num # num -> num) (fext:ext) (si:state_circuit) (s:state_circuit) (a:ag32_state) (t:num) <=>
   (fext.data_in = (FUNPOW Next (I(5,t)) a).data_in) /\
   (** visible part: directly seen by ISA **)
   ((s.EX.EX_carry_flag <=> (FUNPOW Next (I(3,t)) a).CarryFlag)) /\
@@ -229,11 +231,11 @@ Definition Rel_def:
   (s.data_out = (FUNPOW Next (I(5,t)) a).data_out) /\
   (reg_data_vaild 5 s ==> (s.R = (FUNPOW Next (I(5,t)) a).R)) /\
   (** invisible part **)
-  (enable_stg 1 s ==> IF_Rel fext s a (I(1,t))) /\
+  (enable_stg 1 si ==> IF_Rel fext s a (I(1,t))) /\
   (enable_stg 2 s ==> ID_Rel fext s a (I(2,t))) /\
-  (enable_stg 3 s ==> EX_Rel fext s a (I(3,t))) /\
-  (enable_stg 4 s ==> MEM_Rel fext s a (I(4,t))) /\
-  (enable_stg 5 s ==> WB_Rel fext s a (I(5,t)))
+  (enable_stg 3 si ==> EX_Rel fext s a (I(3,t))) /\
+  (enable_stg 4 si ==> MEM_Rel fext s a (I(4,t))) /\
+  (enable_stg 5 si ==> WB_Rel fext s a (I(5,t)))
 End
 
 val _ = export_theory ();
